theories/XTyping.v
@@ -12,75 +12,72 @@ Section XTyping.
 
 Context `{Sort_notion : Sorts.notion}.
 
-Inductive typing (Σ : sglobal_context) : scontext -> sterm -> sterm -> Type :=
-| type_Rel Γ n :
-    wf Σ Γ ->
+Inductive typing (Σ : sglobal_context) (Γ : scontext) : sterm -> sterm -> Type :=
+| type_Rel n :
     forall (isdecl : n < List.length Γ),
       Σ ;;; Γ |-x (sRel n) : lift0 (S n) (safe_nth Γ (exist _ n isdecl))
 
-| type_Sort Γ s :
-    wf Σ Γ ->
+| type_Sort s :
     Σ ;;; Γ |-x (sSort s) : sSort (succ s)
 
-| type_Prod Γ n t b s1 s2 :
+| type_Prod n t b s1 s2 :
     Σ ;;; Γ |-x t : sSort s1 ->
     Σ ;;; Γ ,, t |-x b : sSort s2 ->
     Σ ;;; Γ |-x (sProd n t b) : sSort (Sorts.prod_sort s1 s2)
 
-| type_Lambda Γ n n' t b s1 s2 bty :
+| type_Lambda n n' t b s1 s2 bty :
     Σ ;;; Γ |-x t : sSort s1 ->
     Σ ;;; Γ ,, t |-x bty : sSort s2 ->
     Σ ;;; Γ ,, t |-x b : bty ->
     Σ ;;; Γ |-x (sLambda n t bty b) : sProd n' t bty
 
-| type_App Γ n s1 s2 t A B u :
+| type_App n s1 s2 t A B u :
     Σ ;;; Γ |-x A : sSort s1 ->
     Σ ;;; Γ ,, A |-x B : sSort s2 ->
     Σ ;;; Γ |-x t : sProd n A B ->
     Σ ;;; Γ |-x u : A ->
     Σ ;;; Γ |-x (sApp t A B u) : B{ 0 := u }
 
-| type_Sum Γ n t b s1 s2 :
+| type_Sum n t b s1 s2 :
     Σ ;;; Γ |-x t : sSort s1 ->
     Σ ;;; Γ ,, t |-x b : sSort s2 ->
     Σ ;;; Γ |-x (sSum n t b) : sSort (Sorts.sum_sort s1 s2)
 
-| type_Pair Γ n A B u v s1 s2 :
+| type_Pair n A B u v s1 s2 :
     Σ ;;; Γ |-x A : sSort s1 ->
     Σ ;;; Γ ,, A |-x B : sSort s2 ->
     Σ ;;; Γ |-x u : A ->
     Σ ;;; Γ |-x v : B{ 0 := u } ->
     Σ ;;; Γ |-x sPair A B u v : sSum n A B
 
-| type_Pi1 Γ n A B s1 s2 p :
+| type_Pi1 n A B s1 s2 p :
     Σ ;;; Γ |-x p : sSum n A B ->
     Σ ;;; Γ |-x A : sSort s1 ->
     Σ ;;; Γ ,, A |-x B : sSort s2 ->
     Σ ;;; Γ |-x sPi1 A B p : A
 
-| type_Pi2 Γ n A B s1 s2 p :
+| type_Pi2 n A B s1 s2 p :
     Σ ;;; Γ |-x p : sSum n A B ->
     Σ ;;; Γ |-x A : sSort s1 ->
     Σ ;;; Γ ,, A |-x B : sSort s2 ->
     Σ ;;; Γ |-x sPi2 A B p : B{ 0 := sPi1 A B p }
 
-| type_Eq Γ s A u v :
+| type_Eq s A u v :
     Σ ;;; Γ |-x A : sSort s ->
     Σ ;;; Γ |-x u : A ->
     Σ ;;; Γ |-x v : A ->
     Σ ;;; Γ |-x sEq A u v : sSort (Sorts.eq_sort s)
 
-| type_Refl Γ s A u :
+| type_Refl s A u :
     Σ ;;; Γ |-x A : sSort s ->
     Σ ;;; Γ |-x u : A ->
     Σ ;;; Γ |-x sRefl A u : sEq A u u
 
-| type_Ax Γ id ty :
-    wf Σ Γ ->
+| type_Ax id ty :
     lookup_glob Σ id = Some ty ->
     Σ ;;; Γ |-x sAx id : ty
 
-| type_conv Γ t A B s :
+| type_conv t A B s :
     Σ ;;; Γ |-x t : A ->
     Σ ;;; Γ |-x B : sSort s ->
     Σ ;;; Γ |-x A = B : sSort s ->
@@ -88,50 +85,41 @@ Inductive typing (Σ : sglobal_context) : scontext -> sterm -> sterm -> Type :=
 
 where " Σ ;;; Γ '|-x' t : T " := (@typing Σ Γ t T) : x_scope
 
-with wf (Σ : sglobal_context) : scontext -> Type :=
-| wf_nil :
-    wf Σ nil
-
-| wf_snoc Γ A s :
-    wf Σ Γ ->
-    Σ ;;; Γ |-x A : sSort s ->
-    wf Σ (Γ ,, A)
-
-with eq_term (Σ : sglobal_context) : scontext -> sterm -> sterm -> sterm -> Type :=
-| eq_reflexivity Γ u A :
+with eq_term (Σ : sglobal_context) (Γ : scontext) : sterm -> sterm -> sterm -> Type :=
+| eq_reflexivity u A :
     Σ ;;; Γ |-x u : A ->
     Σ ;;; Γ |-x u = u : A
 
-| eq_symmetry Γ u v A :
+| eq_symmetry u v A :
     Σ ;;; Γ |-x u = v : A ->
     Σ ;;; Γ |-x v = u : A
 
-| eq_transitivity Γ u v w A :
+| eq_transitivity u v w A :
     Σ ;;; Γ |-x u = v : A ->
     Σ ;;; Γ |-x v = w : A ->
     Σ ;;; Γ |-x u = w : A
 
-| eq_beta Γ s1 s2 n A B t u :
+| eq_beta s1 s2 n A B t u :
     Σ ;;; Γ |-x A : sSort s1 ->
     Σ ;;; Γ ,, A |-x B : sSort s2 ->
     Σ ;;; Γ ,, A |-x t : B ->
     Σ ;;; Γ |-x u : A ->
     Σ ;;; Γ |-x sApp (sLambda n A B t) A B u = t{ 0 := u } : B{ 0 := u }
 
-| eq_conv Γ s T1 T2 t1 t2 :
+| eq_conv s T1 T2 t1 t2 :
     Σ ;;; Γ |-x t1 = t2 : T1 ->
     Σ ;;; Γ |-x T1 = T2 : sSort s ->
     Σ ;;; Γ |-x t1 = t2 : T2
 
-| cong_Prod Γ n1 n2 A1 A2 B1 B2 s1 s2 :
+| cong_Prod n1 n2 A1 A2 B1 B2 s1 s2 :
     Σ ;;; Γ |-x A1 = A2 : sSort s1 ->
     Σ ;;; Γ ,, A1 |-x B1 = B2 : sSort s2 ->
     Σ ;;; Γ ,, A1 |-x B1 : sSort s2 ->
     Σ ;;; Γ ,, A2 |-x B2 : sSort s2 ->
-    Σ ;;; Γ |-x (sProd n1 A1 B1) = (sProd n2 A2 B2) : 
+    Σ ;;; Γ |-x (sProd n1 A1 B1) = (sProd n2 A2 B2) :
                sSort (Sorts.prod_sort s1 s2)
 
-| cong_Lambda Γ n1 n2 n' A1 A2 B1 B2 t1 t2 s1 s2 :
+| cong_Lambda n1 n2 n' A1 A2 B1 B2 t1 t2 s1 s2 :
     Σ ;;; Γ |-x A1 = A2 : sSort s1 ->
     Σ ;;; Γ ,, A1 |-x B1 = B2 : sSort s2 ->
     Σ ;;; Γ ,, A1 |-x t1 = t2 : B1 ->
@@ -141,7 +129,7 @@ with eq_term (Σ : sglobal_context) : scontext -> sterm -> sterm -> sterm -> Typ
     Σ ;;; Γ ,, A2 |-x t2 : B2 ->
     Σ ;;; Γ |-x (sLambda n1 A1 B1 t1) = (sLambda n2 A2 B2 t2) : sProd n' A1 B1
 
-| cong_App Γ n1 n2 s1 s2 t1 t2 A1 A2 B1 B2 u1 u2 :
+| cong_App n1 n2 s1 s2 t1 t2 A1 A2 B1 B2 u1 u2 :
     Σ ;;; Γ |-x A1 = A2 : sSort s1 ->
     Σ ;;; Γ ,, A1 |-x B1 = B2 : sSort s2 ->
     Σ ;;; Γ |-x t1 = t2 : sProd n1 A1 B1 ->
@@ -154,14 +142,14 @@ with eq_term (Σ : sglobal_context) : scontext -> sterm -> sterm -> sterm -> Typ
     Σ ;;; Γ |-x u2 : A2 ->
     Σ ;;; Γ |-x (sApp t1 A1 B1 u1) = (sApp t2 A2 B2 u2) : B1{ 0 := u1 }
 
-| cong_Sum Γ n1 n2 A1 A2 B1 B2 s1 s2 :
+| cong_Sum n1 n2 A1 A2 B1 B2 s1 s2 :
     Σ ;;; Γ |-x A1 = A2 : sSort s1 ->
     Σ ;;; Γ ,, A1 |-x B1 = B2 : sSort s2 ->
     Σ ;;; Γ ,, A1 |-x B1 : sSort s2 ->
     Σ ;;; Γ ,, A2 |-x B2 : sSort s2 ->
     Σ ;;; Γ |-x (sSum n1 A1 B1) = (sSum n2 A2 B2) : sSort (Sorts.sum_sort s1 s2)
 
-| cong_Pair Γ n A1 A2 B1 B2 u1 u2 v1 v2 s1 s2 :
+| cong_Pair n A1 A2 B1 B2 u1 u2 v1 v2 s1 s2 :
     Σ ;;; Γ |-x A1 = A2 : sSort s1 ->
     Σ ;;; Γ ,, A1 |-x B1 = B2 : sSort s2 ->
     Σ ;;; Γ |-x u1 = u2 : A1 ->
@@ -174,7 +162,7 @@ with eq_term (Σ : sglobal_context) : scontext -> sterm -> sterm -> sterm -> Typ
     Σ ;;; Γ |-x v2 : B2{ 0 := u2 } ->
     Σ ;;; Γ |-x sPair A1 B1 u1 v1 = sPair A2 B2 u2 v2 : sSum n A1 B1
 
-| cong_Pi1 Γ nx ny A1 A2 B1 B2 s1 s2 p1 p2 :
+| cong_Pi1 nx ny A1 A2 B1 B2 s1 s2 p1 p2 :
     Σ ;;; Γ |-x p1 = p2 : sSum nx A1 B1 ->
     Σ ;;; Γ |-x A1 = A2 : sSort s1 ->
     Σ ;;; Γ ,, A1 |-x B1 = B2 : sSort s2 ->
@@ -184,7 +172,7 @@ with eq_term (Σ : sglobal_context) : scontext -> sterm -> sterm -> sterm -> Typ
     Σ ;;; Γ |-x p2 : sSum ny A2 B2 ->
     Σ ;;; Γ |-x sPi1 A1 B1 p1 = sPi1 A2 B2 p2 : A1
 
-| cong_Pi2 Γ nx ny A1 A2 B1 B2 s1 s2 p1 p2 :
+| cong_Pi2 nx ny A1 A2 B1 B2 s1 s2 p1 p2 :
     Σ ;;; Γ |-x p1 = p2 : sSum nx A1 B1 ->
     Σ ;;; Γ |-x A1 = A2 : sSort s1 ->
     Σ ;;; Γ ,, A1 |-x B1 = B2 : sSort s2 ->
@@ -194,38 +182,39 @@ with eq_term (Σ : sglobal_context) : scontext -> sterm -> sterm -> sterm -> Typ
     Σ ;;; Γ |-x p2 : sSum ny A2 B2 ->
     Σ ;;; Γ |-x sPi2 A1 B1 p1 = sPi2 A2 B2 p2 : B1{ 0 := sPi1 A1 B1 p1 }
 
-| cong_Eq Γ s A1 A2 u1 u2 v1 v2 :
+| cong_Eq s A1 A2 u1 u2 v1 v2 :
     Σ ;;; Γ |-x A1 = A2 : sSort s ->
     Σ ;;; Γ |-x u1 = u2 : A1 ->
     Σ ;;; Γ |-x v1 = v2 : A1 ->
     Σ ;;; Γ |-x sEq A1 u1 v1 = sEq A2 u2 v2 : sSort (Sorts.eq_sort s)
 
-| cong_Refl Γ s A1 A2 u1 u2 :
+| cong_Refl s A1 A2 u1 u2 :
     Σ ;;; Γ |-x A1 = A2 : sSort s ->
     Σ ;;; Γ |-x u1 = u2 : A1 ->
     Σ ;;; Γ |-x sRefl A1 u1 = sRefl A2 u2 : sEq A1 u1 u1
 
-| reflection Γ A u v e :
+| reflection A u v e :
     Σ ;;; Γ |-x e : sEq A u v ->
     Σ ;;; Γ |-x u = v : A
 
 where " Σ ;;; Γ '|-x' t = u : T " := (@eq_term Σ Γ t u T) : x_scope.
 
-Derive Signature for typing.
-Derive Signature for wf.
-Derive Signature for eq_term.
-
 Delimit Scope x_scope with x.
 
 Open Scope x_scope.
 
-Lemma typing_wf :
-  forall {Σ Γ t T},
-    Σ ;;; Γ |-x t : T ->
-    wf Σ Γ.
-Proof.
-  intros Σ Γ t T H. induction H ; easy.
-Defined.
+Inductive wf (Σ : sglobal_context) : scontext -> Type :=
+| wf_nil :
+    wf Σ nil
+
+| wf_snoc Γ A s :
+    wf Σ Γ ->
+    Σ ;;; Γ |-x A : sSort s ->
+    wf Σ (Γ ,, A).
+
+Derive Signature for typing.
+Derive Signature for wf.
+Derive Signature for eq_term.
 
 End XTyping.
 
