theories/XChecking.v
@@ -11,129 +11,114 @@ From Translation Require Import util Quotes Sorts SAst SLiftSubst SCommon
 (* For efficiency reasons we use type in type for examples. *)
 Existing Instance Sorts.type_in_type.
 
-(* Lemma type_conv'' : *)
-(*   forall {Γ t A B s}, *)
-(*     Σi ;;; Γ |-x t : A -> *)
-(*     Σi ;;; Γ |-x A = B : sSort s -> *)
-(*     Σi ;;; Γ |-x B : sSort s -> *)
-(*     Σi ;;; Γ |-x t : B. *)
-(* Proof. *)
-(*   intros Γ t A B s H H0 H1. *)
-(*   eapply type_conv ; eassumption. *)
-(* Defined. *)
-
+(* Even when not necessary, we require wf Σ Γ so that we can propagate
+   the information that the context is indeed well-formed.
+ *)
 
 Lemma xtype_Prod' :
   forall {Σ Γ n A B},
+    wf Σ Γ ->
     Σ ;;; Γ |-x A : Ty ->
     (wf Σ (Γ ,, A) -> Σ ;;; Γ ,, A |-x B : Ty) ->
     Σ ;;; Γ |-x sProd n A B : Ty.
 Proof.
-  intros Σ Γ n A B hA hB.
-  eapply meta_conv.
-  - eapply type_Prod.
-    + eassumption.
-    + apply hB. econstructor ; try eassumption.
-      eapply typing_wf. eassumption.
-  - reflexivity.
+  intros Σ Γ n A B hw hA hB.
+  assert (hwA : wf Σ (Γ ,, A)).
+  { econstructor ; eassumption. }
+  specialize (hB hwA).
+  eapply type_Prod with (s1 := tt) (s2 := tt) ; assumption.
 Defined.
 
 Lemma xtype_Lambda' :
   forall {Σ Γ n n' A B t},
     xtype_glob Σ ->
+    wf Σ Γ ->
     Σ ;;; Γ |-x A : Ty ->
-    (wf Σ (Γ ,, A) -> Σ ;;; Γ ,, A |-x t : B) ->
+    (wf Σ (Γ,, A) -> Σ ;;; Γ ,, A |-x t : B) ->
     Σ ;;; Γ |-x sLambda n A B t : sProd n' A B.
 Proof.
-  intros Σ Γ n n' A B t xhg hA ht.
-  assert (hw : wf Σ (Γ ,, A)).
-  { econstructor ; try eassumption.
-    eapply typing_wf. eassumption.
-  }
-  specialize (ht hw).
-  destruct (istype_type xhg ht) as [[] hB].
+  intros Σ Γ n n' A B t xhg hw hA ht.
+  assert (hwA : wf Σ (Γ ,, A)).
+  { econstructor ; eassumption. }
+  specialize (ht hwA).
+  destruct (istype_type xhg hwA ht) as [[] hB].
   eapply type_Lambda ; eassumption.
 Defined.
 
 Lemma xtype_App' :
   forall {Σ Γ n t A B u},
     xtype_glob Σ ->
+    wf Σ Γ ->
     Σ ;;; Γ |-x t : sProd n A B ->
     Σ ;;; Γ |-x u : A ->
     Σ ;;; Γ |-x sApp t A B u : (B{0 := u})%s.
 Proof.
-  intros Σ Γ n t A B u xhg ht hu.
-  destruct (istype_type xhg hu) as [[] hA].
-  destruct (istype_type xhg ht) as [[] hPi].
-  assert (hw : wf Σ (Γ ,, A)).
-  { econstructor ; try eassumption.
-    eapply typing_wf. eassumption.
-  }
+  intros Σ Γ n t A B u xhg hw ht hu.
+  destruct (istype_type xhg hw hu) as [[] hA].
+  destruct (istype_type xhg hw ht) as [[] hPi].
+  assert (hwA : wf Σ (Γ ,, A)).
+  { econstructor ; eassumption. }
   destruct (inversionProd hPi) as [[? ?] ?].
   eapply type_App ; eassumption.
 Defined.
 
 Lemma xtype_Sum' :
   forall {Σ Γ n A B},
+    wf Σ Γ ->
     Σ ;;; Γ |-x A : Ty ->
     (wf Σ (Γ ,, A) -> Σ ;;; Γ ,, A |-x B : Ty) ->
     Σ ;;; Γ |-x sSum n A B : Ty.
 Proof.
-  intros Σ Γ n A B hA hB.
-  eapply meta_conv.
-  - eapply type_Sum.
-    + eassumption.
-    + apply hB. econstructor ; try eassumption.
-      eapply typing_wf. eassumption.
-  - reflexivity.
+  intros Σ Γ n A B hw hA hB.
+  assert (hwA : wf Σ (Γ ,, A)).
+  { econstructor ; eassumption. }
+  specialize (hB hwA).
+  eapply type_Sum with (s1 := tt) (s2 := tt) ; assumption.
 Defined.
 
 Lemma xtype_Eq' :
   forall {Σ Γ A u v},
     xtype_glob Σ ->
+    wf Σ Γ ->
     Σ ;;; Γ |-x u : A ->
     Σ ;;; Γ |-x v : A ->
     Σ ;;; Γ |-x sEq A u v : Ty.
 Proof.
-  intros Σ Γ A u v xhg hu hv.
-  destruct (istype_type xhg hu) as [[] hA].
-  eapply meta_conv.
-  - eapply type_Eq ; eassumption.
-  - reflexivity.
+  intros Σ Γ A u v xhg hw hu hv.
+  destruct (istype_type xhg hw hu) as [[] hA].
+  eapply type_Eq with (s := tt) ; assumption.
 Defined.
 
 Lemma xtype_Refl' :
   forall {Σ Γ A u},
     xtype_glob Σ ->
+    wf Σ Γ ->
     Σ ;;; Γ |-x u : A ->
     Σ ;;; Γ |-x sRefl A u : sEq A u u.
 Proof.
-  intros Σ Γ A u xhg hu.
-  destruct (istype_type xhg hu) as [[] hA].
+  intros Σ Γ A u xhg hw hu.
+  destruct (istype_type xhg hw hu) as [[] hA].
   eapply type_Refl ; eassumption.
 Defined.
 
 Lemma xtype_Sort' :
   forall {Σ Γ},
-    wf Σ Γ ->
     Σ ;;; Γ |-x Ty : Ty.
 Proof.
-  intros Σ Γ h.
-  eapply meta_conv.
-  - eapply type_Sort. assumption.
-  - reflexivity.
+  intros Σ Γ.
+  eapply type_Sort with (s := tt).
 Defined.
 
-Lemma xwf_snoc' :
-  forall {Σ Γ A},
-    Σ ;;; Γ |-x A : Ty ->
-    wf Σ (Γ ,, A).
-Proof.
-  intros Σ Γ A h.
-  econstructor.
-  - eapply typing_wf. eassumption.
-  - eassumption.
-Defined.
+(* Lemma xwf_snoc' : *)
+(*   forall {Σ Γ A}, *)
+(*     Σ ;;; Γ |-x A : Ty -> *)
+(*     wf Σ (Γ ,, A). *)
+(* Proof. *)
+(*   intros Σ Γ A h. *)
+(*   econstructor. *)
+(*   - eapply typing_wf. eassumption. *)
+(*   - eassumption. *)
+(* Defined. *)
 
 Lemma xtype_glob_cons' :
   forall {Σ d},
@@ -161,18 +146,18 @@ Ltac ettintro Σi :=
   lazymatch goal with
   | |- ?Σ ;;; ?Γ |-x ?t : ?T =>
     lazymatch t with
-    | sRel ?n => refine (@type_Rel Sorts.type_in_type _ _ n _ _)
+    | sRel ?n => refine (@type_Rel Sorts.type_in_type _ _ n _)
     | sSort _ => eapply xtype_Sort'
-    | sProd _ _ _ => eapply xtype_Prod' ; [| intro ]
+    | sProd _ _ _ => eapply xtype_Prod' ; [ .. | intro ]
     | sLambda _ _ _ _ => eapply xtype_Lambda' ; [ .. | intro ]
     | sApp _ _ _ _ => eapply xtype_App'
-    | sSum _ _ _ => eapply xtype_Sum' ; [| intro ]
+    | sSum _ _ _ => eapply xtype_Sum' ; [ .. | intro ]
     | sPair _ _ _ _ => eapply type_Pair
     | sPi1 _ _ _ => eapply type_Pi1
     | sPi2 _ _ _ => eapply type_Pi2
     | sEq _ _ _ => eapply xtype_Eq'
     | sRefl _ _ => eapply xtype_Refl'
-    | sAx _ => eapply type_Ax ; [| lazy - [Σi]; try reflexivity ]
+    | sAx _ => eapply type_Ax ; lazy - [Σi] ; try reflexivity
     | _ => fail "No introduction rule for" t
     end
   | _ => fail "Not applicable"
@@ -182,14 +167,14 @@ Ltac ettcheck1 Σi :=
   lazymatch goal with
   | |- ?Σ ;;; ?Γ |-x ?t : ?T =>
     first [
-      eapply meta_conv ; [ ettintro Σi |   lazy - [Σi] ; reflexivity ]
+      eapply meta_conv ; [ ettintro Σi | lazy - [Σi] ; reflexivity ]
     | eapply type_conv ; [ ettintro Σi | .. ]
     (* | eapply meta_ctx_conv ; [ *)
     (*     eapply meta_conv ; [ ettintro | lazy ; try reflexivity ] *)
     (*   | cbn ; try reflexivity *)
     (*   ] *)
     ]
-  | |- wf ?Σ ?Γ => first [ assumption | eapply xwf_snoc' | econstructor ]
+  | |- wf ?Σ ?Γ => first [ assumption | econstructor ]
   | |- sSort _ = sSort _ => first [ lazy - [Σi]  ; reflexivity | shelve ]
   | |- type_glob _ => first [ assumption | glob Σi]
   | |- xtype_glob _ => first [ assumption | xglob Σi ]
